design a reset register.
This is really cool. HOL caught my design error. It is fixed in version
2, which is still not perfect, because it contains an unnecessary
component, ONE.

parity/parityTheory.sig
@@ -1,0 +1,92 @@
+signature parityTheory =
+sig
+  type thm = Thm.thm
+
+  (*  Definitions  *)
+    val MUX_def : thm
+    val NOT_def : thm
+    val ONE_def : thm
+    val PARITY_IMP_def : thm
+    val PARITY_def : thm
+    val REG_def : thm
+
+  (*  Theorems  *)
+    val PARITY_CORRECT : thm
+    val PARITY_LEMMA : thm
+    val PARITY_def_compute : thm
+    val UNIQUENESS_LEMMA : thm
+
+  val parity_grammars : type_grammar.grammar * term_grammar.grammar
+(*
+   [quantHeuristics] Parent theory of "parity"
+
+   [rich_list] Parent theory of "parity"
+
+   [MUX_def]  Definition
+
+      |- ∀sw in1 in2 out.
+           MUX (sw,in1,in2,out) ⇔ ∀t. out t ⇔ if sw t then in1 t else in2 t
+
+   [NOT_def]  Definition
+
+      |- ∀inp out. NOT (inp,out) ⇔ ∀t. out t ⇔ ¬inp t
+
+   [ONE_def]  Definition
+
+      |- ∀out. ONE out ⇔ ∀t. out t ⇔ T
+
+   [PARITY_IMP_def]  Definition
+
+      |- ∀inp out.
+           PARITY_IMP (inp,out) ⇔
+           ∃l1 l2 l3 l4 l5.
+             NOT (l2,l1) ∧ MUX (inp,l1,l2,l3) ∧ MUX (l5,l3,l4,out) ∧
+             ONE l4 ∧ REG (l4,l5) ∧ REG (out,l2)
+
+   [PARITY_def]  Definition
+
+      |- (∀input. PARITY 0 input ⇔ T) ∧
+         ∀t input.
+           PARITY (SUC t) input ⇔
+           if input (SUC t) then ¬PARITY t input else PARITY t input
+
+   [REG_def]  Definition
+
+      |- ∀inp out.
+           REG (inp,out) ⇔ ∀t. out t ⇔ if t = 0 then F else inp (t − 1)
+
+   [PARITY_CORRECT]  Theorem
+
+      |- ∀inp out. PARITY_IMP (inp,out) ⇒ ∀t. out t ⇔ PARITY t inp
+
+   [PARITY_LEMMA]  Theorem
+
+      |- ∀inp out.
+           PARITY_IMP (inp,out) ⇒
+           (out 0 ⇔ T) ∧
+           ∀t. out (SUC t) ⇔ if inp (SUC t) then ¬out t else out t
+
+   [PARITY_def_compute]  Theorem
+
+      |- (∀input. PARITY 0 input ⇔ T) ∧
+         (∀t input.
+            PARITY (NUMERAL (BIT1 t)) input ⇔
+            if input (NUMERAL (BIT1 t)) then
+              ¬PARITY (NUMERAL (BIT1 t) − 1) input
+            else PARITY (NUMERAL (BIT1 t) − 1) input) ∧
+         ∀t input.
+           PARITY (NUMERAL (BIT2 t)) input ⇔
+           if input (NUMERAL (BIT2 t)) then
+             ¬PARITY (NUMERAL (BIT1 t)) input
+           else PARITY (NUMERAL (BIT1 t)) input
+
+   [UNIQUENESS_LEMMA]  Theorem
+
+      |- ∀inp out.
+           (out 0 ⇔ T) ∧
+           (∀t. out (SUC t) ⇔ if inp (SUC t) then ¬out t else out t) ⇒
+           ∀t. out t ⇔ PARITY t inp
+
+
+*)
+end
