parity/parityScript.sml
@@ -1,4 +1,9 @@
-open arithmeticTheory;
+
+open HolKernel boolLib Parse bossLib
+
+
+
+val _ = new_theory "parity"
 
 val PARITY_def = Define `(PARITY 0 input = T) /\ (PARITY (SUC t) input = if input (SUC t) then ~ (PARITY t input) else PARITY t input)`;
 
@@ -8,6 +13,51 @@ val SPECIFICATION = ``!t. out t = PARITY t input``;
 
 (* lemma *)
 
-val lemma = store_thm("lemma",
- `` !input out. (out 0 = T) /\ (!t. out (SUC t) = (if input (SUC t) then ~(out t) else out t) ) ==> !t. out t = PARITY t input ``,
- REPEAT GEN_TAC THEN STRIP_TAC THEN Induct THEN  ASM_REWRITE_TAC [PARITY_def] THEN  ASM_REWRITE_TAC [PARITY_def]);
+val UNIQUENESS_LEMMA = store_thm(
+  "UNIQUENESS_LEMMA",
+  ``!inp out.
+      (out 0 = T) /\
+      (!t. out (SUC t) = if inp (SUC t) then ~out t else out t)
+         ==>
+      !t. out t = PARITY t inp``,
+  REPEAT GEN_TAC THEN STRIP_TAC THEN Induct THENL [
+    ASM_REWRITE_TAC [PARITY_def],
+    ASM_REWRITE_TAC [PARITY_def]
+  ]);
+
+
+(* Definition of circuit components *)
+val ONE_def = Define `ONE (out:num->bool) = !t. out t = T`;
+val NOT_def = Define `NOT (inp,out:num->bool) = !t. out t = ~ (inp t)`;
+val MUX_def = Define `MUX (sw,in1,in2, out:num->bool) = !t. out t = if sw t then in1 t else in2 t`;
+val REG_def = Define `REG (inp,out:num->bool) = !t. out t = if t = 0 then F else inp (t-1)`;
+
+(* Parity Implementation *)
+val PARITY_IMP_def = Define `PARITY_IMP (inp, out) = ?l1 l2 l3 l4 l5. NOT(l2,l1) /\ MUX(inp,l1,l2,l3) /\ MUX(l5,l3,l4,out) /\ ONE(l4) /\ REG(l4,l5) /\ REG(out,l2)`;
+
+(* Verification *)
+
+val PARITY_LEMMA = store_thm("PARITY_LEMMA",
+  ``!inp out.
+        PARITY_IMP(inp,out)
+           ==>
+        (out 0 = T) /\
+        !t. out(SUC t) = if inp(SUC t) then ~(out t) else out t``,
+  PURE_REWRITE_TAC [PARITY_IMP_def, ONE_def, NOT_def, MUX_def, REG_def] THEN
+  REPEAT STRIP_TAC THENL [
+    PROVE_TAC [],
+    PAT_ASSUM ``!t. out t = X t``
+              (fn th => REWRITE_TAC [SPEC ``SUC t`` th]) THEN
+    RW_TAC arith_ss []
+  ]);
+
+val PARITY_CORRECT = store_thm(
+  "PARITY_CORRECT",
+    ``!inp out. PARITY_IMP(inp,out)
+                   ==>
+                !t. out t = PARITY t inp``,
+    RW_TAC std_ss []
+      THEN MATCH_MP_TAC UNIQUENESS_LEMMA
+      THEN PROVE_TAC [PARITY_LEMMA]);
+
+val _ = export_theory()
